\tiny
$\begin{array}{rll}
-4 & \text{Import}~                           & \vdash \forall x, z. (x \in \mathcal{U}(z)) \Leftrightarrow \exists y. (x \in y) \land (y \in z) \\
-3 & \text{Import}~                           & \vdash \forall x, y. (\forall z. (z \in x) \Leftrightarrow (z \in y)) \Leftrightarrow (x = y) \\
-2 & \text{Import}~                           & \vdash \forall x, y. (x \subseteq y) \Leftrightarrow \forall z. (z \in x) \Rightarrow (z \in y) \\
-1 & \text{Import}~                           & \vdash \forall x, y. (x \in \mathcal{P}(y)) \Leftrightarrow (x \subseteq y) \\
 0 & \text{Hypo.}~                            & \forall z. ({?s} \in \mathcal{U}(z)) \Leftrightarrow \exists y. ({?s} \in y) \land (y \in z) \vdash \forall z. ({?s} \in \mathcal{U}(z)) \Leftrightarrow \exists y. ({?s} \in y) \land (y \in z) \\
 1 & \text{Left}~{\forall}~0                  & \forall x, z. (x \in \mathcal{U}(z)) \Leftrightarrow \exists y. (x \in y) \land (y \in z) \vdash \forall z. ({?s} \in \mathcal{U}(z)) \Leftrightarrow \exists y. ({?s} \in y) \land (y \in z) \\
 2 & \text{Cut}~{-4}, 1                       & \vdash \forall z. ({?s} \in \mathcal{U}(z)) \Leftrightarrow \exists y. ({?s} \in y) \land (y \in z) \\
 3 & \text{Hypo.}~                            & ({?s} \in \mathcal{U}({?t})) \Leftrightarrow \exists y. ({?s} \in y) \land (y \in {?t}) \vdash ({?s} \in \mathcal{U}({?t})) \Leftrightarrow \exists y. ({?s} \in y) \land (y \in {?t}) \\
 4 & \text{Left}~{\forall}~3                  & \forall z. ({?s} \in \mathcal{U}(z)) \Leftrightarrow \exists y. ({?s} \in y) \land (y \in z) \vdash ({?s} \in \mathcal{U}({?t})) \Leftrightarrow \exists y. ({?s} \in y) \land (y \in {?t}) \\
 5 & \text{Cut}~2, 4                          & \vdash ({?s} \in \mathcal{U}({?t})) \Leftrightarrow \exists y. ({?s} \in y) \land (y \in {?t}) \\
 6 & \text{Hypo.}~                            & \forall y. ({?s} \in \mathcal{P}(y)) \Leftrightarrow ({?s} \subseteq y) \vdash \forall y. ({?s} \in \mathcal{P}(y)) \Leftrightarrow ({?s} \subseteq y) \\
 7 & \text{Left}~{\forall}~6                  & \forall x, y. (x \in \mathcal{P}(y)) \Leftrightarrow (x \subseteq y) \vdash \forall y. ({?s} \in \mathcal{P}(y)) \Leftrightarrow ({?s} \subseteq y) \\
 8 & \text{Cut}~{-1}, 7                       & \vdash \forall y. ({?s} \in \mathcal{P}(y)) \Leftrightarrow ({?s} \subseteq y) \\
 9 & \text{Hypo.}~                            & ({?s} \in \mathcal{P}({?t})) \Leftrightarrow ({?s} \subseteq {?t}) \vdash ({?s} \in \mathcal{P}({?t})) \Leftrightarrow ({?s} \subseteq {?t}) \\
10 & \text{Left}~{\forall}~9                  & \forall y. ({?s} \in \mathcal{P}(y)) \Leftrightarrow ({?s} \subseteq y) \vdash ({?s} \in \mathcal{P}({?t})) \Leftrightarrow ({?s} \subseteq {?t}) \\
11 & \text{Cut}~8, 10                         & \vdash ({?s} \in \mathcal{P}({?t})) \Leftrightarrow ({?s} \subseteq {?t}) \\
12 & \text{Hypo.}~                            & \forall y. ({?s} \subseteq y) \Leftrightarrow \forall z. (z \in {?s}) \Rightarrow (z \in y) \vdash \forall y. ({?s} \subseteq y) \Leftrightarrow \forall z. (z \in {?s}) \Rightarrow (z \in y) \\
13 & \text{Left}~{\forall}~12                 & \forall x, y. (x \subseteq y) \Leftrightarrow \forall z. (z \in x) \Rightarrow (z \in y) \vdash \forall y. ({?s} \subseteq y) \Leftrightarrow \forall z. (z \in {?s}) \Rightarrow (z \in y) \\
14 & \text{Cut}~{-2}, 13                      & \vdash \forall y. ({?s} \subseteq y) \Leftrightarrow \forall z. (z \in {?s}) \Rightarrow (z \in y) \\
15 & \text{Hypo.}~                            & ({?s} \subseteq {?t}) \Leftrightarrow \forall z. (z \in {?s}) \Rightarrow (z \in {?t}) \vdash ({?s} \subseteq {?t}) \Leftrightarrow \forall z. (z \in {?s}) \Rightarrow (z \in {?t}) \\
16 & \text{Left}~{\forall}~15                 & \forall y. ({?s} \subseteq y) \Leftrightarrow \forall z. (z \in {?s}) \Rightarrow (z \in y) \vdash ({?s} \subseteq {?t}) \Leftrightarrow \forall z. (z \in {?s}) \Rightarrow (z \in {?t}) \\
17 & \text{Cut}~14, 16                        & \vdash ({?s} \subseteq {?t}) \Leftrightarrow \forall z. (z \in {?s}) \Rightarrow (z \in {?t}) \\
18 & \text{Hypo.}~                            & {?v} \in {?s} \vdash {?v} \in {?s} \\
19 & \text{Right}~{\Rightarrow}~18            & \vdash ({?v} \in {?s}) \Rightarrow ({?v} \in {?s}) \\
20 & \text{Rewrite}~19                        & \setminus z. \vdash (z \in {?s}) \Rightarrow (z \in {?s}) \\
21 & \text{Right}~{\forall}~20                & \vdash \forall z. (z \in {?s}) \Rightarrow (z \in {?s}) \\
22 & \text{Rewrite}~21                        & ({?t} \in {?s}) \Rightarrow ({?t} \in {?s}) \vdash \forall z. (z \in {?s}) \Rightarrow (z \in {?s}) \\
23 & \text{Right}~{\Rightarrow}~22            & \vdash (({?t} \in {?s}) \Rightarrow ({?t} \in {?s})) \Rightarrow \forall z. (z \in {?s}) \Rightarrow (z \in {?s}) \\
24 & \text{Hypo.}~                            & ({?t} \in {?s}) \Rightarrow ({?t} \in {?s}) \vdash ({?t} \in {?s}) \Rightarrow ({?t} \in {?s}) \\
25 & \text{Left}~{\forall}~24                 & \forall z. (z \in {?s}) \Rightarrow (z \in {?s}) \vdash ({?t} \in {?s}) \Rightarrow ({?t} \in {?s}) \\
26 & \text{Right}~{\Rightarrow}~25            & \vdash (\forall z. (z \in {?s}) \Rightarrow (z \in {?s})) \Rightarrow ({?t} \in {?s}) \Rightarrow ({?t} \in {?s}) \\
27 & \text{Right}~{\Leftrightarrow}~26, 23    & \vdash (\forall z. (z \in {?s}) \Rightarrow (z \in {?s})) \Leftrightarrow ({?t} \in {?s}) \Rightarrow ({?t} \in {?s}) \\
28 & \text{?Fun. Instantiation}~17            & \vdash ({?s} \subseteq {?s}) \Leftrightarrow \forall z. (z \in {?s}) \Rightarrow (z \in {?s}) \\
29 & \text{Rewrite}~28                        & \vdash (\forall z. (z \in {?s}) \Rightarrow (z \in {?s})) \Leftrightarrow ({?s} \subseteq {?s}) \\
30 & \text{Right Subst.}~{\Leftrightarrow}~27 & (\forall z. (z \in {?s}) \Rightarrow (z \in {?s})) \Leftrightarrow ({?s} \subseteq {?s}) \vdash ({?s} \subseteq {?s}) \Leftrightarrow ({?t} \in {?s}) \Rightarrow ({?t} \in {?s}) \\
31 & \text{Cut}~29, 30                        & \vdash ({?s} \subseteq {?s}) \Leftrightarrow ({?t} \in {?s}) \Rightarrow ({?t} \in {?s}) \\
32 & \text{Hypo.}~                            & \forall y. (\forall z. (z \in {?s}) \Leftrightarrow (z \in y)) \Leftrightarrow ({?s} = y) \vdash \forall y. (\forall z. (z \in {?s}) \Leftrightarrow (z \in y)) \Leftrightarrow ({?s} = y) \\
33 & \text{Left}~{\forall}~32                 & \forall x, y. (\forall z. (z \in x) \Leftrightarrow (z \in y)) \Leftrightarrow (x = y) \vdash \forall y. (\forall z. (z \in {?s}) \Leftrightarrow (z \in y)) \Leftrightarrow ({?s} = y) \\
34 & \text{Cut}~{-3}, 33                      & \vdash \forall y. (\forall z. (z \in {?s}) \Leftrightarrow (z \in y)) \Leftrightarrow ({?s} = y) \\
35 & \text{Hypo.}~                            & (\forall z. (z \in {?s}) \Leftrightarrow (z \in {?t})) \Leftrightarrow ({?s} = {?t}) \vdash (\forall z. (z \in {?s}) \Leftrightarrow (z \in {?t})) \Leftrightarrow ({?s} = {?t}) \\
36 & \text{Left}~{\forall}~35                 & \forall y. (\forall z. (z \in {?s}) \Leftrightarrow (z \in y)) \Leftrightarrow ({?s} = y) \vdash (\forall z. (z \in {?s}) \Leftrightarrow (z \in {?t})) \Leftrightarrow ({?s} = {?t}) \\
37 & \text{Cut}~34, 36                        & \vdash (\forall z. (z \in {?s}) \Leftrightarrow (z \in {?t})) \Leftrightarrow ({?s} = {?t}) \\
38 & \text{?Fun. Instantiation}~37            & \vdash (\forall z. (z \in {?s}) \Leftrightarrow (z \in \mathcal{U}(\mathcal{P}({?s})))) \Leftrightarrow ({?s} = \mathcal{U}(\mathcal{P}({?s}))) \\
39 & \text{Rewrite}~38                        & \vdash (\forall z. (z \in \mathcal{U}(\mathcal{P}({?s}))) \Leftrightarrow (z \in {?s})) \Leftrightarrow (\mathcal{U}(\mathcal{P}({?s})) = {?s}) \\
40 & \text{Hypo.}~                            & {?t} \in {?s} \vdash {?t} \in {?s} \\
41 & \text{Right}~{\Rightarrow}~40            & {?t} \in {?s} \vdash ({?t} \in {?s}) \Rightarrow ({?t} \in {?s}) \\
42 & \text{Weakening}~31                      & {?t} \in {?s} \vdash ({?t} \in {?s}) \Rightarrow ({?t} \in {?s}) \Leftrightarrow ({?s} \subseteq {?s}) \\
43 & \text{Right Subst.}~{\Leftrightarrow}~41 & ({?t} \in {?s}) \Rightarrow ({?t} \in {?s}) \Leftrightarrow ({?s} \subseteq {?s}); {?t} \in {?s} \vdash {?s} \subseteq {?s} \\
44 & \text{Cut}~42, 43                        & {?t} \in {?s} \vdash {?s} \subseteq {?s} \\
45 & \text{?Fun. Instantiation}~11            & \vdash ({?s} \in \mathcal{P}({?s})) \Leftrightarrow ({?s} \subseteq {?s}) \\
46 & \text{Weakening}~45                      & {?t} \in {?s} \vdash ({?s} \subseteq {?s}) \Leftrightarrow ({?s} \in \mathcal{P}({?s})) \\
47 & \text{Right Subst.}~{\Leftrightarrow}~44 & ({?s} \subseteq {?s}) \Leftrightarrow ({?s} \in \mathcal{P}({?s})); {?t} \in {?s} \vdash {?s} \in \mathcal{P}({?s}) \\
48 & \text{Cut}~46, 47                        & {?t} \in {?s} \vdash {?s} \in \mathcal{P}({?s}) \\
49 & \text{Right}~{\land}~40, 48              & {?t} \in {?s} \vdash ({?t} \in {?s}) \land ({?s} \in \mathcal{P}({?s})) \\
50 & \text{Right}~{\exists}~49                & {?t} \in {?s} \vdash \exists y. ({?t} \in y) \land (y \in \mathcal{P}({?s})) \\
51 & \text{Right}~{\Rightarrow}~50            & \vdash ({?t} \in {?s}) \Rightarrow \exists y. ({?t} \in y) \land (y \in \mathcal{P}({?s})) \\
52 & \text{Hypo.}~                            & {?t} \in {?s}; {?t} \in {?u} \vdash {?t} \in {?s} \\
53 & \text{Hypo.}~                            & {?t} \in {?u} \vdash {?t} \in {?s}; {?t} \in {?u} \\
54 & \text{Left}~{\Rightarrow}~53, 52         & ({?t} \in {?u}) \Rightarrow ({?t} \in {?s}); {?t} \in {?u} \vdash {?t} \in {?s} \\
55 & \text{Left}~{\forall}~54                 & \forall z. (z \in {?u}) \Rightarrow (z \in {?s}); {?t} \in {?u} \vdash {?t} \in {?s} \\
56 & \text{?Fun. Instantiation}~17            & \vdash ({?u} \subseteq {?s}) \Leftrightarrow \forall z. (z \in {?u}) \Rightarrow (z \in {?s}) \\
57 & \text{Weakening}~56                      & {?t} \in {?u} \vdash (\forall z. (z \in {?u}) \Rightarrow (z \in {?s})) \Leftrightarrow ({?u} \subseteq {?s}); {?t} \in {?s} \\
58 & \text{Left Subst.}~{\Leftrightarrow}~55  & (\forall z. (z \in {?u}) \Rightarrow (z \in {?s})) \Leftrightarrow ({?u} \subseteq {?s}); {?t} \in {?u}; {?u} \subseteq {?s} \vdash {?t} \in {?s} \\
59 & \text{Cut}~57, 58                        & {?t} \in {?u}; {?u} \subseteq {?s} \vdash {?t} \in {?s} \\
60 & \text{?Fun. Instantiation}~11            & \vdash ({?u} \in \mathcal{P}({?s})) \Leftrightarrow ({?u} \subseteq {?s}) \\
61 & \text{Weakening}~60                      & {?t} \in {?u} \vdash ({?u} \subseteq {?s}) \Leftrightarrow ({?u} \in \mathcal{P}({?s})); {?t} \in {?s} \\
62 & \text{Left Subst.}~{\Leftrightarrow}~59  & ({?u} \subseteq {?s}) \Leftrightarrow ({?u} \in \mathcal{P}({?s})); {?t} \in {?u}; {?u} \in \mathcal{P}({?s}) \vdash {?t} \in {?s} \\
63 & \text{Cut}~61, 62                        & {?t} \in {?u}; {?u} \in \mathcal{P}({?s}) \vdash {?t} \in {?s} \\
64 & \text{Left}~{\land}~63                   & ({?t} \in {?u}) \land ({?u} \in \mathcal{P}({?s})) \vdash {?t} \in {?s} \\
65 & \text{?Fun. Instantiation}~64            & \setminus y. ({?t} \in y) \land (y \in \mathcal{P}({?s})) \vdash {?t} \in {?s} \\
66 & \text{Left}~{\exists}~65                 & \exists y. ({?t} \in y) \land (y \in \mathcal{P}({?s})) \vdash {?t} \in {?s} \\
67 & \text{Right}~{\Rightarrow}~66            & \vdash (\exists y. ({?t} \in y) \land (y \in \mathcal{P}({?s}))) \Rightarrow ({?t} \in {?s}) \\
68 & \text{Right}~{\Leftrightarrow}~67, 51    & \vdash (\exists y. ({?t} \in y) \land (y \in \mathcal{P}({?s}))) \Leftrightarrow ({?t} \in {?s}) \\
69 & \text{?Fun. Instantiation}~5             & \vdash ({?t} \in \mathcal{U}(\mathcal{P}({?s}))) \Leftrightarrow \exists y. ({?t} \in y) \land (y \in \mathcal{P}({?s})) \\
70 & \text{Right Subst.}~{\Leftrightarrow}~69 & (\exists y. ({?t} \in y) \land (y \in \mathcal{P}({?s}))) \Leftrightarrow ({?t} \in {?s}) \vdash ({?t} \in \mathcal{U}(\mathcal{P}({?s}))) \Leftrightarrow ({?t} \in {?s}) \\
71 & \text{Cut}~68, 70                        & \vdash ({?t} \in \mathcal{U}(\mathcal{P}({?s}))) \Leftrightarrow ({?t} \in {?s}) \\
72 & \text{?Fun. Instantiation}~71            & \setminus z. \vdash (z \in \mathcal{U}(\mathcal{P}({?s}))) \Leftrightarrow (z \in {?s}) \\
73 & \text{Right}~{\forall}~72                & \vdash \forall z. (z \in \mathcal{U}(\mathcal{P}({?s}))) \Leftrightarrow (z \in {?s}) \\
74 & \text{Right Subst.}~{\Leftrightarrow}~73 & (\forall z. (z \in \mathcal{U}(\mathcal{P}({?s}))) \Leftrightarrow (z \in {?s})) \Leftrightarrow (\mathcal{U}(\mathcal{P}({?s})) = {?s}) \vdash \mathcal{U}(\mathcal{P}({?s})) = {?s} \\
75 & \text{Cut}~39, 74                        & \vdash \mathcal{U}(\mathcal{P}({?s})) = {?s}
\end{array}$
\normalsize