\section{Appendix}

\newcommand{\frule}[3]{
  \begin{prooftree}
  \hypo{#1}
  \infer1[(#3)]{#2}
  \end{prooftree}
}

\begin{figure}[H]
  \begin{framed}
  $$\arraycolsep=0.75cm\def\arraystretch{2.75}\begin{array}{c c}
  % Hypothesis
  \frule{}{{?a} \vdash {?a}}{H.} & \\
  % And
  \frule{{?a}, {?b} \vdash}{{?a} \land {?b} \vdash}{I.L.$\land$} & \frule{\vdash {?a} \quad \vdash {?b}}{\vdash {?a} \land {?b}}{I.R.$\land$} \\
  \frule{{?a} \land {?b} \vdash}{{?a}, {?b} \vdash}{E.L.$\land$} & \frule{\vdash {?a} \land {?b}}{\vdash {?a}}{E.R.$\land_1$} \\ % cont.
  & \frule{\vdash {?a} \land {?b}}{\vdash {?b}}{E.R.$\land_2$} \\
  % Or
  \frule{{?a} \vdash \quad {?b} \vdash}{{?a} \lor {?b} \vdash}{I.L.$\lor$} & \frule{\vdash {?a}, {?b}}{\vdash {?a} \lor {?b}}{I.R.$\lor$} \\
  \frule{{?a} \lor {?b} \vdash}{{?a} \vdash}{E.L.$\lor_1$} & \frule{\vdash {?a} \lor {?b}}{\vdash {?a}, {?b}}{E.R.$\lor$} \\ % cont.
  \frule{{?a} \lor {?b} \vdash}{{?b} \vdash}{E.L.$\lor_2$} & \\
  % Implies
  \frule{\vdash {?a} \quad {?b} \vdash}{{?a} \Rightarrow {?b} \vdash}{I.L.$\Rightarrow$} & \frule{{?a} \vdash {?b}}{\vdash {?a} \Rightarrow {?b}}{I.R.$\Rightarrow$} \\
  \frule{{?a} \Rightarrow {?b} \vdash}{\vdash {?a}}{E.L.$\Rightarrow_1$} & \frule{\vdash {?a} \Rightarrow {?b}}{{?a} \vdash {?b}}{E.R.$\Rightarrow$} \\ % cont.
  \frule{{?a} \Rightarrow {?b} \vdash}{{?b} \vdash}{E.L.$\Rightarrow_2$} & \\
  % Iff
  \frule{{?a} \Rightarrow {?b}, {?b} \Rightarrow {?a} \vdash}{{?a} \Leftrightarrow {?b} \vdash}{I.L.$\Leftrightarrow$} & \frule{\vdash {?a} \Rightarrow {?b} \quad \vdash {?b} \Rightarrow {?a}}{\vdash {?a} \Leftrightarrow {?b}}{I.R.$\Leftrightarrow$} \\
  \frule{{?a} \Leftrightarrow {?b} \vdash}{{?a} \Rightarrow {?b}, {?b} \Rightarrow {?a} \vdash}{E.L.$\Leftrightarrow$} & \frule{\vdash {?a} \Leftrightarrow {?b}}{\vdash {?a} \Rightarrow {?b}}{E.R.$\Leftrightarrow_1$} \\ % cont.
  & \frule{\vdash {?a} \Leftrightarrow {?b}}{\vdash {?b} \Rightarrow {?a}}{E.R.$\Leftrightarrow_2$}
  \end{array}$$
  \end{framed}
  \caption[Rules (1)]{Predefined rules provided in the front. For clarity, contexts have been omitted: the intended semantic is the one described in \autoref{sec:proof-framework-rules}. ``H'', ``I'', ``E'', ``L'' and ``R'' respectively stand for ``Hypothesis'', ``Introduction'', ``Elimination'', ``Left'' and ``Right''. In the source, shorthand for these names are used, for instance ``I.L.$\land$'' would be identified by \code{introLAnd}. Most introduction rules map to a single kernel proof step. Elimination rules on the other hand rely on the cut rule.}
  \label{fig:rules-list-1}
\end{figure}

\begin{figure}[H]
\begin{framed}
  $$\arraycolsep=0.75cm\def\arraystretch{3}\begin{array}{c c}
  % Not
  \frule{\vdash {?a}}{\neg {?a} \vdash}{I.L.$\neg$} & \frule{{?a} \vdash}{\vdash \neg {?a}}{I.R.$\neg$} \\
  \frule{\neg {?a} \vdash}{\vdash {?a}}{E.L.$\neg$} & \frule{\vdash \neg {?a}}{{?a} \vdash}{E.R.$\neg$} \\
  % Eq. refl.
  \frule{{?s} = {?s} \vdash}{\vdash}{E.L.$=$} & \frule{}{\vdash {?s} = {?s}}{I.R.$=$} \\
  % Forall
  \frule{{?p}({?t}) \vdash}{\forall x. {?p}(x) \vdash}{I.L.$\forall$} & \frule{\vdash {?p}(\overline{?t})}{\vdash \forall x. {?p}(x)}{I.R.$\forall$} \\
  \frule{\forall x. {?p}(x) \vdash}{{?p}({?t}) \vdash}{E.L.$\forall$} & \frule{\vdash \forall x. {?p}(x)}{\vdash {?p}(\overline{?t})}{E.R.$\forall$} \\
  % Exists
  \frule{{?p}(\overline{?t}) \vdash}{\exists x. {?p}(x) \vdash}{I.L.$\exists$} & \frule{\vdash {?p}({?t})}{\vdash \exists x. {?p}(x)}{I.R.$\exists$} \\
  \frule{\exists x. {?p}(x) \vdash}{{?p}(\overline{?t}) \vdash}{E.L.$\exists$} & \frule{\vdash \exists x. {?p}(x)}{\vdash {?p}({?t})}{E.R.$\exists$} \\
  % Iff subst.
  \frule{{?f}({?a}) \vdash}{{?a} \Leftrightarrow {?b}, {?f}({?b}) \vdash}{I.L.S.$\Leftrightarrow$} & \frule{\vdash {?f}({?a}) \quad}{{?a} \Leftrightarrow {?b} \vdash {?f}({?b})}{I.R.S.$\Leftrightarrow$} \\
  \frule{{?f}({?a}) \vdash \quad \vdash {?a} \Leftrightarrow {?b}}{{?f}({?b}) \vdash}{E.L.S.$\Leftrightarrow$} & \frule{\vdash {?f}({?a}) \quad \vdash {?a} \Leftrightarrow {?b}}{\vdash {?f}({?b})}{E.R.S.$\Leftrightarrow$} \\
  % Eq. subst.
  \frule{{?p}({?s}) \vdash \quad}{{?s} = {?t}, {?p}({?t}) \vdash}{I.L.S.$=$} & \frule{\vdash {?p}({?s})}{{?s} = {?t} \vdash {?p}({?t})}{I.R.S.$=$} \\
  \frule{{?p}({?s}) \vdash \quad \vdash {?s} = {?t}}{{?p}({?t}) \vdash}{E.L.S.$=$} & \frule{\vdash {?p}({?s}) \quad \vdash {?s} = {?t}}{\vdash {?p}({?t})}{E.R.S.$=$}
  \end{array}$$
  \end{framed}
  \caption[Rules (2)]{Continuation of \autoref{fig:rules-list-1}. Schemas marked with an overline are constrained to resolve to fresh schemas; namely schemas that do not appear elsewhere in the sequent, apart from this binding.}
  \label{fig:rules-list-2}
\end{figure}

\input{figures/proof-sample.scala}

\begin{figure}[H]
  \centering
  \input{figures/proof-sample.lisa.tex}
  \caption[Sample proof (kernel)]{Example of a generated kernel proof following its description in the front (\autoref{fig:scala-proof-sample}). This proof is independent of any theory but depends on the axiom of powerset, the definition of the subset relation and the axioms of extensionality and union (imports 1-4). Such a kernel proof is objectively difficult to be produced by hand; in contrast it is relatively straightforward to be achieved in the front. Note that the latex code used in this figure is also part of the output.}
  \label{fig:lisa-proof-sample}
\end{figure}
